add miller rabin exe and refactor zmodpow

PrimalityTests/ZModPow.lean
@@ -6,33 +6,33 @@ import Mathlib.Data.ZMod.Basic
 
 namespace ZMod
 
-example (n : ZMod 10) : n ^ 5 = n := by fin_cases n <;> rfl
-
 /-- Fast modular exponentiation, tail recursive -/
-def pow {n : ℕ} (x : ZMod n) (m : ℕ) (y : ZMod n := 1) : ZMod n :=
-  match m with
-  | 0 => y
-  | m + 1 => (x * x).pow (m.succ / 2) (x ^ (m.succ % 2) * y)
-termination_by _ x m y => m
-decreasing_by
-  simp_wf
-  exact m.div_lt_self' 0
+def pow {n : ℕ} (m : ℕ) (x : ZMod n) : ZMod n :=
+  go m x 1
+where
+  go (m : ℕ) (x y : ZMod n) : ZMod n :=
+    match m with
+    | 0 => y
+    | m + 1 => go (m.succ / 2) (x * x) (x ^ (m.succ % 2) * y)
+  termination_by _ n m x y => m
+  decreasing_by
+    simp_wf
+    exact m.div_lt_self' 0
 
-theorem pow_eq' {n : ℕ} (x : ZMod n) (m : ℕ) (y : ZMod n) : x.pow m y = x ^ m * y := by
-  unfold pow
+theorem pow.go_eq {n m : ℕ} {x y : ZMod n} : pow.go m x y = x ^ m * y := by
+  unfold pow.go
   cases m with
   | zero => rw [Nat.zero_eq, _root_.pow_zero, one_mul]
   | succ m =>
-    dsimp
-    rw [pow_eq' (x * x) (m.succ / 2) (x ^ (m.succ % 2) * y), ← mul_assoc, ← pow_two,
-      ← pow_mul, ← pow_add, Nat.div_add_mod]
-termination_by _ x m y => m
+    dsimp only
+    rw [pow.go_eq, ← mul_assoc, ← pow_two, ← pow_mul, ← pow_add, Nat.div_add_mod]
+termination_by _ n m x y => m
 decreasing_by
   simp_wf
   exact n.div_lt_self' 0
 
-theorem pow_eq {n : ℕ} (x : ZMod n) (m : ℕ) : x.pow m = x ^ m :=
-  by rw [pow_eq' x m 1, mul_one]
+theorem pow_eq {n : ℕ} {x : ZMod n} {m : ℕ} : x.pow m = x ^ m :=
+  by rw [pow, pow.go_eq, mul_one]
 
 #eval (5 : ZMod 8972345).pow 198092436098975768588789
 
