PrimalityTests/MillerRabin.lean
@@ -1,3 +1,4 @@
+import Cli
 import Init.Data.Random
 import PrimalityTests.StrongProbable
 
@@ -8,21 +9,25 @@ import PrimalityTests.StrongProbable
 /-- The *Miller–Rabin* primality test on input `n`, run `r` times. -/
 def millerRabin {gen : Type*} [RandomGen gen] (g : gen) (n r : ℕ) :
     Bool × gen :=
-  match r with
-  | Nat.zero => (true, g)
-  | Nat.succ r =>
-    if n ≤ 1 then
-      (false, g)
-    else if n = 2 then
-      (true, g)
-    else if 2 ∣ n then
-      (false, g)
-    else
-      let (a, g') := randNat g 1 (n - 1)
-      if SPP n (a : ZMod n) then
-        millerRabin g' n r
-      else
-        (false, g')
+  if n ≤ 1 then
+    (false, g)
+  else if n = 2 then
+    (true, g)
+  else if 2 ∣ n then
+    (false, g)
+  else
+    go r
+    where
+      v := val₂ (n - 1)
+      o := oddPart (n - 1)
+      go : ℕ → Bool × gen
+      | Nat.zero => (true, g)
+      | Nat.succ r =>
+          let (a, g') := randNat g 1 (n - 1)
+          if SPP.loopMulSelf v ((a : ZMod n).pow o) = none then
+            millerRabin g' n r
+          else
+            (false, g')
 
 /-- Runs Miller–Rabin on `n`, `r` times.
 Uses `StdGen` (so obviously don't use for cryptographic purposes). -/
@@ -35,6 +40,50 @@ def runMillerRabin (n r : ℕ) : IO Bool := do
 -- 9 is the strongest pseudoprime
 #eval runMillerRabin 9 1  -- this is true 1/4 of the times
 #eval runMillerRabin 9 10 -- this is false almost definitely
+
+section Cli
+
+open Cli
+
+def runExhaustiveTest (p : Parsed) : IO UInt32 := do
+  let n := p.positionalArg! "n" |>.as! Nat
+  let v := val₂ (n - 1)
+  let o := oddPart (n - 1)
+  for a in List.range'TR 1 (n - 1) do
+    let _ := SPP.loopMulSelf v ((a : ZMod n).pow o)
+  return 0
+
+def runMillerRabinCmd (p : Parsed) : IO UInt32 := do
+  let n := p.positionalArg! "n" |>.as! Nat
+  let r := p.positionalArg! "r" |>.as! Nat
+  let res ← runMillerRabin n r
+  IO.println <| if res then "prime" else "composite"
+  return 0
+
+def exhaustiveTestCmd := `[Cli|
+  "exhaustive-test" VIA runExhaustiveTest;
+  "Tests Miller–Rabin for all bases 0 < a < n."
+
+  ARGS:
+    n : Nat; "The candidate prime."
+]
+
+def millerRabinCmd := `[Cli|
+  "miller-rabin" VIA runMillerRabinCmd;
+  "Tests primality of a number using the Miller–Rabin primality test."
+
+  ARGS:
+    n : Nat; "The candidate prime."
+    r : Nat; "Number of repeats."
+
+  SUBCOMMANDS:
+    exhaustiveTestCmd
+]
+
+end Cli
+
+def main (args : List String) : IO UInt32 := do
+  millerRabinCmd.validate args
 
 /-!
 Then one should be able to prove millerRabin is correct with prob. 1 - 4⁻ʳ,
