lakefile.lean
@@ -1,14 +1,13 @@
 import Lake
 open Lake DSL
 
-package «primality_tests» {
-  -- add any package configuration options here
-}
+package «primality-tests»
 
 require mathlib from git
   "https://github.com/leanprover-community/mathlib4.git"
 
 @[default_target]
-lean_lib «PrimalityTests» {
-  -- add any library configuration options here
-}
+lean_lib PrimalityTests
+
+lean_exe «miller-rabin» where
+  root := `PrimalityTests.MillerRabin
